src/Parsers/ContextFreeGrammar/Notations.v
@@ -19,14 +19,14 @@ Definition list_to_productions {T} (default : T) (ls : list (string * T)) : stri
   := fun nt
      => option_rect
           (fun _ => T)
-          (fun idx => nth idx (map snd ls) default)
+          (fun idx => nth idx (map snd (uniquize (fun x y => string_beq (fst x) (fst y)) ls)) default)
           default
-          (first_index_error (string_beq nt) (map fst ls)).
+          (first_index_error (string_beq nt) (uniquize string_beq (map fst ls))).
 
 Definition list_to_grammar {T} (default : productions T) (ls : list (string * productions T)) : grammar T
-  := {| Start_symbol := hd ""%string (map fst ls);
+  := {| Start_symbol := hd ""%string (uniquize string_beq (map fst ls));
         Lookup := list_to_productions default ls;
-        Valid_nonterminals := map fst ls |}.
+        Valid_nonterminals := uniquize string_beq (map fst ls) |}.
 
 Definition item_ascii := item Ascii.ascii.
 Coercion item_of_char (ch : Ascii.ascii) : item_ascii := Terminal ch.
