src/Parsers/Refinement/ReductionTactics.v
@@ -32,7 +32,8 @@ Declare Reduction parser_red8 := simpl @snd.
 Declare Reduction parser_red9 := simpl List.length.
 Declare Reduction parser_red10 := simpl List.fold_right.
 Declare Reduction parser_red11 := simpl @Operations.first_index_error.
-Declare Reduction parser_red12 := cbv beta iota zeta delta [Fix2 Fix2_F].
+Declare Reduction parser_red12 := simpl @Operations.up_to.
+Declare Reduction parser_red13 := cbv beta iota zeta delta [Fix2 Fix2_F].
 
 Ltac parser_red term :=
   let term := match term with
@@ -54,6 +55,7 @@ Ltac parser_red term :=
   let term := (eval parser_red10 in term) in
   let term := (eval parser_red11 in term) in
   let term := (eval parser_red12 in term) in
+  let term := (eval parser_red13 in term) in
   constr:term.
 
 Class eq_refl_vm_cast T := by_vm_cast : T.
